Revert "Make the types of the finite map type classes more specific."
This reverts commit 20b4ae55bdf00edb751ccdab3eb876cb9b13c99f, which does
not seem to work with Coq 8.5pl2 (I accidentally tested with 8.5pl1).

algebra/list.v
@@ -17,17 +17,17 @@ Global Instance tail_ne n : Proper (dist n ==> dist n) (@tail A) := _.
 Global Instance take_ne n : Proper (dist n ==> dist n) (@take A n) := _.
 Global Instance drop_ne n : Proper (dist n ==> dist n) (@drop A n) := _.
 Global Instance list_lookup_ne n i :
-  Proper (dist n ==> dist n) (lookup (M:=list) i).
+  Proper (dist n ==> dist n) (lookup (M:=list A) i).
 Proof. intros ???. by apply dist_option_Forall2, Forall2_lookup. Qed.
 Global Instance list_alter_ne n f i :
   Proper (dist n ==> dist n) f →
-  Proper (dist n ==> dist n) (alter (M:=list) f i) := _.
+  Proper (dist n ==> dist n) (alter (M:=list A) f i) := _.
 Global Instance list_insert_ne n i :
-  Proper (dist n ==> dist n ==> dist n) (insert (M:=list) i) := _.
+  Proper (dist n ==> dist n ==> dist n) (insert (M:=list A) i) := _.
 Global Instance list_inserts_ne n i :
   Proper (dist n ==> dist n ==> dist n) (@list_inserts A i) := _.
 Global Instance list_delete_ne n i :
-  Proper (dist n ==> dist n) (delete (M:=list) i) := _.
+  Proper (dist n ==> dist n) (delete (M:=list A) i) := _.
 Global Instance option_list_ne n : Proper (dist n ==> dist n) (@option_list A).
 Proof. intros ???; by apply Forall2_option_list, dist_option_Forall2. Qed.
 Global Instance list_filter_ne n P `{∀ x, Decision (P x)} :
@@ -236,20 +236,17 @@ End cmra.
 Arguments listR : clear implicits.
 Arguments listUR : clear implicits.
 
-Definition list_singleton {A : ucmraT} (n : nat) (x : A) : list A :=
+Instance list_singletonM {A : ucmraT} : SingletonM nat A (list A) := λ n x,
   replicate n ∅ ++ [x].
 
 Section properties.
   Context {A : ucmraT}.
-  Implicit Types l k : list A.
-  Implicit Types ml mk : option (list A).
+  Implicit Types l : list A.
   Implicit Types x y z : A.
-  Implicit Types i : nat.
   Local Arguments op _ _ !_ !_ / : simpl nomatch.
   Local Arguments cmra_op _ !_ !_ / : simpl nomatch.
 
-  Lemma list_lookup_opM l mk i :
-    (l ⋅? mk) !! i = l !! i ⋅ (mk ≫= (!! i) : option A).
+  Lemma list_lookup_opM l mk i : (l ⋅? mk) !! i = l !! i ⋅ (mk ≫= (!! i)).
   Proof. destruct mk; by rewrite /= ?list_lookup_op ?right_id_L. Qed.
 
   Lemma list_op_app l1 l2 l3 :
@@ -269,52 +266,57 @@ Section properties.
 
   Lemma replicate_valid n (x : A) : ✓ x → ✓ replicate n x.
   Proof. apply Forall_replicate. Qed.
-  Global Instance list_singleton_ne n i :
-    Proper (dist n ==> dist n) (@list_singleton A i).
+  Global Instance list_singletonM_ne n i :
+    Proper (dist n ==> dist n) (@list_singletonM A i).
   Proof. intros l1 l2 ?. apply Forall2_app; by repeat constructor. Qed.
-  Global Instance list_singleton_proper i :
-    Proper ((≡) ==> (≡)) (list_singleton i) := ne_proper _.
+  Global Instance list_singletonM_proper i :
+    Proper ((≡) ==> (≡)) (list_singletonM i) := ne_proper _.
 
-  Lemma elem_of_list_singleton i z x : z ∈ list_singleton i x → z = ∅ ∨ z = x.
+  Lemma elem_of_list_singletonM i z x : z ∈ {[i := x]} → z = ∅ ∨ z = x.
   Proof.
     rewrite elem_of_app elem_of_list_singleton elem_of_replicate. naive_solver.
   Qed.
-  Lemma list_lookup_singleton i x : list_singleton i x !! i = Some x.
+  Lemma list_lookup_singletonM i x : {[ i := x ]} !! i = Some x.
   Proof. induction i; by f_equal/=. Qed.
-  Lemma list_lookup_singleton_ne i j x :
-    i ≠ j → list_singleton i x !! j = None ∨ list_singleton i x !! j = Some ∅.
+  Lemma list_lookup_singletonM_ne i j x :
+    i ≠ j → {[ i := x ]} !! j = None ∨ {[ i := x ]} !! j = Some ∅.
   Proof. revert j; induction i; intros [|j]; naive_solver auto with omega. Qed.
-  Lemma list_singleton_validN n i x : ✓{n} (list_singleton i x) ↔ ✓{n} x.
+  Lemma list_singletonM_validN n i x : ✓{n} {[ i := x ]} ↔ ✓{n} x.
   Proof.
     rewrite list_lookup_validN. split.
-    { move=> /(_ i). by rewrite list_lookup_singleton. }
+    { move=> /(_ i). by rewrite list_lookup_singletonM. }
     intros Hx j; destruct (decide (i = j)); subst.
-    - by rewrite list_lookup_singleton.
-    - destruct (list_lookup_singleton_ne i j x) as [Hi|Hi]; first done;
+    - by rewrite list_lookup_singletonM.
+    - destruct (list_lookup_singletonM_ne i j x) as [Hi|Hi]; first done;
         rewrite Hi; by try apply (ucmra_unit_validN (A:=A)).
   Qed.
-  Lemma list_singleton_valid  i x : ✓ (list_singleton i x) ↔ ✓ x.
+  Lemma list_singleton_valid  i x : ✓ {[ i := x ]} ↔ ✓ x.
   Proof.
-    rewrite !cmra_valid_validN. by setoid_rewrite list_singleton_validN.
+    rewrite !cmra_valid_validN. by setoid_rewrite list_singletonM_validN.
   Qed.
-  Lemma list_singleton_length i x : length (list_singleton i x) = S i.
-  Proof. rewrite /list_singleton app_length replicate_length /=; lia. Qed.
-
-  Lemma list_core_singleton i x :
-    core (list_singleton i x) ≡ list_singleton i (core x).
+  Lemma list_singletonM_length i x : length {[ i := x ]} = S i.
   Proof.
-    rewrite /list_singleton.
+    rewrite /singletonM /list_singletonM app_length replicate_length /=; lia.
+  Qed.
+
+  Lemma list_core_singletonM i (x : A) : core {[ i := x ]} ≡ {[ i := core x ]}.
+  Proof.
+    rewrite /singletonM /list_singletonM.
     by rewrite {1}/core /= fmap_app fmap_replicate (persistent_core ∅).
   Qed.
-  Lemma list_op_singleton i x y :
-    list_singleton i x ⋅ list_singleton i y ≡ list_singleton i (x ⋅ y).
-  Proof. induction i; constructor; rewrite ?left_id; auto. Qed.
-  Lemma list_alter_singleton f i x :
-    alter f i (list_singleton i x) = list_singleton i (f x).
-  Proof. rewrite /list_singleton. induction i; f_equal/=; auto. Qed.
-  Global Instance list_singleton_persistent i x :
-    Persistent x → Persistent (list_singleton i x).
-  Proof. by rewrite !persistent_total list_core_singleton=> ->. Qed.
+  Lemma list_op_singletonM i (x y : A) :
+    {[ i := x ]} ⋅ {[ i := y ]} ≡ {[ i := x ⋅ y ]}.
+  Proof.
+    rewrite /singletonM /list_singletonM /=.
+    induction i; constructor; rewrite ?left_id; auto.
+  Qed.
+  Lemma list_alter_singletonM f i x : alter f i {[i := x]} = {[i := f x]}.
+  Proof.
+    rewrite /singletonM /list_singletonM /=. induction i; f_equal/=; auto.
+  Qed.
+  Global Instance list_singleton_persistent i (x : A) :
+    Persistent x → Persistent {[ i := x ]}.
+  Proof. by rewrite !persistent_total list_core_singletonM=> ->. Qed.
 
   (* Update *)
   Lemma list_middle_updateP (P : A → Prop) (Q : list A → Prop) l1 x l2 :
@@ -360,7 +362,7 @@ Section properties.
   Qed.
 
   Lemma list_singleton_local_update i x y ml :
-    x ~l~> y @ ml ≫= (!! i) → list_singleton i x ~l~> list_singleton i y @ ml.
+    x ~l~> y @ ml ≫= (!! i) → {[ i := x ]} ~l~> {[ i := y ]} @ ml.
   Proof. intros; apply list_middle_local_update. by rewrite replicate_length. Qed.
 End properties.
 
